pushed TV through EM -> DM, now just callstate matching left for that pass

src/Emajortodmajor.v
@@ -389,6 +389,7 @@ Inductive match_cont: Emajor.cont -> Dmajor.cont -> mem -> Prop :=
       match_cont (Emajor.Kblock k) (Dmajor.Kblock k') m
 | match_cont_seq: forall s s' k k' m,
     transf_stmt s = s' ->
+    lists_ok s = true ->
     match_cont k k' m ->
     match_cont (Emajor.Kseq s k) (Dmajor.Kseq s' k') m
 | match_cont_call: forall id f e k f' e' k' m,
@@ -403,6 +404,7 @@ Inductive match_states: Emajor.state -> Dmajor.state -> Prop :=
     forall f f' s s' k k' e e' m,
       transf_function f = OK f' ->
       transf_stmt s = s' ->
+      lists_ok s = true ->
       match_cont k k' m ->
       env_inject e e' tge m ->
       match_states (Emajor.State f s k e) (Dmajor.State f' s' k' e' m)
@@ -1400,10 +1402,10 @@ Proof.
     app transf_expr_inject (Emajor.eval_expr e earg).
     app symbols_transf Genv.find_symbol.
     app functions_transf Genv.find_funct_ptr.
-    destruct x1; simpl in H15; try congruence.
+    destruct x1; simpl in H16; try congruence.
     Focus 2. unfold bind in *. break_match_hyp; try congruence.
     
-  inv H6. find_rewrite. inv H20.
+  inv H7. find_rewrite. inv H21.
   eexists. split.
   eapply plus_one.
   econstructor; eauto.
@@ -1411,11 +1413,11 @@ Proof.
   econstructor; eauto.
   econstructor; eauto.
   econstructor.
-  simpl. find_rewrite. inv H12.
+  simpl. find_rewrite. inv H13.
   break_match; try congruence.
   eassumption.
-  simpl. find_rewrite. inv H12.
-  unfold bind in *. break_match_hyp; try congruence. inv H15.
+  simpl. find_rewrite. inv H13.
+  unfold bind in *. break_match_hyp; try congruence. inv H16.
   destruct fn; destruct f0; unfold transf_function in Heqr; simpl in Heqr.
   repeat break_match_hyp; try congruence. simpl. inv Heqr. simpl in H13.
   assumption.
@@ -1423,7 +1425,7 @@ Proof.
   unfold bind in *. break_match_hyp; try congruence.
   
   (* return *)
-  + destruct k; simpl in H9; try solve [inv H9]; invp match_cont.
+  + destruct k; simpl in H10; try solve [inv H10]; invp match_cont.
     app transf_expr_inject Emajor.eval_expr.
     eexists; split.
     eapply plus_one.
@@ -1445,16 +1447,16 @@ Proof.
   eapply plus_one.
   econstructor; eauto.
   econstructor; eauto.
+  simpl in H3. break_match_hyp; try congruence.
   econstructor; eauto.
+  simpl in H3. break_match_hyp; try congruence.
 
   (* make_constr *)
   + eapply SmakeConstr_sim; eauto.
-    
-    (* need fact that lists in program aren't too long *)
 
-    (* need a sort of code_of_prog definition *)
-    (* and a proof that whatever we step to is from the prog *)
-    admit.
+    simpl in H3. break_match_hyp; try congruence.
+    intros. eapply bound_spec; eauto. omega.
+    
     
   (* make close *)
   (* same as make constr *)
@@ -1462,8 +1464,8 @@ Proof.
     app functions_transf Genv.find_funct_ptr.
     eapply SmakeClose_sim; eauto.
 
-  (* need fact that lists in program aren't too long *)
-    admit.
+    simpl in H3. break_match_hyp; try congruence.
+    intros. eapply bound_spec; eauto. omega.
 
   (* switch *)
   + app transf_expr_inject Emajor.eval_expr.
@@ -1527,6 +1529,8 @@ Proof.
   unfold transf_function in H1. simpl in H1. repeat break_match_hyp; try congruence.
   unfold transf_function in H1. simpl in H1. inv H1. simpl. reflexivity.
 
+  unfold transf_function in H1. repeat break_match_hyp; try congruence.
+  
   app env_inject_set_params_locals list_forall2.
   unfold transf_function in H1. repeat break_match_hyp; try congruence.
   assert (Emajor.fn_params f = fn_params f').
@@ -1550,9 +1554,7 @@ Proof.
   econstructor; eauto.
   econstructor; eauto.
   simpl. eapply env_inject_update; eauto.
-  
-
-Admitted.
+Qed.  
 
 (* Easier to prove originally with no trace, now just thin wrapper *)
 Lemma step_sim :
@@ -1581,164 +1583,6 @@ Proof.
   eauto.
 Qed.
 
-
-Section ALLOC.
-
-Variable m1: mem.
-Variables lo hi: Z.
-Variable m2: mem.
-Variable b: block.
-Hypothesis ALLOC: Mem.alloc m1 lo hi = (m2, b).
-
-
-Lemma alloc_access_result :
-  Mem.mem_access m2 = PMap.set (Mem.nextblock m1)
-                           (fun (ofs : Z) (_ : perm_kind) =>
-                              if zle lo ofs && zlt ofs hi then Some Freeable else None)
-                           (Mem.mem_access m1).
-Proof.
-  intros.
-  unfold alloc in *. inv ALLOC.
-  simpl. reflexivity.
-Qed.
-
-End ALLOC.
-
-Lemma alloc_drop :
-  forall m lo hi b m',
-    Mem.alloc m lo hi = (m',b) ->
-    forall k m0,
-      Mem.mem_access m' = Mem.mem_access m0 ->
-      exists m'',
-        Mem.drop_perm m0 b lo hi k = Some m''.
-Proof.
-  intros. app alloc_access_result Mem.alloc.
-  rewrite H0 in H. clear H0.
-  unfold Mem.drop_perm.
-  break_match; try solve [eauto].
-  exfalso. apply n.
-  unfold Mem.range_perm.
-  intros.
-  unfold Mem.perm.
-  unfold Mem.perm_order'.
-  rewrite H.
-  app Mem.alloc_result Mem.alloc.
-  subst. rewrite PMap.gss.
-  unfold proj_sumbool. unfold andb.
-  repeat break_match; try congruence; try omega. inv Heqo.
-  econstructor.
-Qed.
-
-(*
-Lemma store_zeros_succeeds :
-  forall m b lo hi,
-    (forall ofs, lo <= ofs < hi -> Mem.valid_access m Mint8unsigned b ofs Writable) ->
-    exists m',
-      store_zeros m b lo hi = Some m' /\ Mem.mem_access m = Mem.mem_access m'.
-Proof.
-Admitted.
-
-Lemma alloc_global_succeeds :
-  forall {F V} (ge : Genv.t F V) a m,
-  exists m',
-    Genv.alloc_global ge m a = Some m'.
-Proof.
-  intros. destruct a.
-  simpl. destruct g.
-  break_let. eapply alloc_drop; eauto.
-  break_let. remember (Genv.init_data_list_size (gvar_init v)) as hi.
-  assert (forall ofs, 0 <= ofs < hi -> Mem.valid_access m0 Mint8unsigned b ofs Writable).
-  intros.
-  eapply Mem.valid_access_implies.
-  eapply Mem.valid_access_alloc_same; eauto; try omega. simpl. omega.
-  simpl. eapply Z.divide_1_l.
-  econstructor.
-  edestruct store_zeros_succeeds; repeat break_and; try rewrite H0; eauto.
-
-  
-Lemma store_init_data_list_succeeds :
-  forall m b lo hi,
-    (forall ofs, lo <= ofs < hi -> Mem.valid_access m Mint8unsigned b ofs Writable) ->
-    exists m',
-      store_zeros m b lo hi = Some m' /\ Mem.mem_access m = Mem.mem_access m'.
-Proof.
-Admitted.
-*)  
-  
-
-Lemma alloc_global_succeeds :
-  forall {F V} (ge : Genv.t F V) id f m,
-  exists m',
-    Genv.alloc_global ge m (id,Gfun f) = Some m'.
-Proof.
-  intros.
-  simpl. 
-  break_let. eapply alloc_drop; eauto.
-Qed.
-
-(* This is true but needs translation validation *)
-Lemma prog_defs_funs :
-  forall id g,
-    In (id,g) (prog_defs tprog) ->
-    exists f,
-      g = Gfun f.
-Proof.
-Admitted.
-
-Lemma alloc_globals_funs_succeeds :
-  forall l m,
-  (forall id g, In (id,g) l -> (exists f, g = Gfun f)) ->
-  exists m',
-    Genv.alloc_globals tge m l = Some m'.
-Proof.
-  induction l; intros.
-  simpl. eauto.
-  simpl.
-  assert (In a (a :: l)). simpl. left. auto.
-  destruct a. eapply H in H0. break_exists. subst g.
-  edestruct (alloc_global_succeeds tge); eauto.
-  rewrite H0.
-  eapply IHl. intros. eapply H. simpl. right. eauto.
-Qed.
-
-Lemma init_mem_succeeds :
-  exists m,
-    Genv.init_mem tprog = Some m.
-Proof.
-  unfold Genv.init_mem.
-  edestruct alloc_globals_funs_succeeds; eauto.
-  eapply prog_defs_funs.
-Qed.
-
-(* Probably need to just validate this, no big deal *)
-Lemma funsig_main :
-  forall b f f',
-    Genv.find_symbol ge (prog_main prog) = Some b ->
-    Genv.find_funct_ptr ge b = Some (Internal f) ->
-    transf_function f = OK f' ->
-    funsig f' = signature_main.
-Proof.
-Admitted.
-
-(*Lemma initial_states_match :
-  forall st,
-    Emajor.initial_state prog st ->
-    exists st',
-      Dmajor.initial_state tprog st' /\ match_states st st'.
-Proof.
-  intros. inv H.
-  destruct init_mem_succeeds.
-  app functions_transf Genv.find_funct_ptr.
-  unfold tge in *. 
-  destruct x0; simpl in H4; unfold bind in *; simpl in H4; break_match_hyp; try congruence.
-  inv H4.
-  eexists; split; repeat (econstructor; eauto).
-  unfold transf_prog in *.
-  erewrite transform_partial_program_main; eauto.
-  eapply symbols_transf; eauto.
-  eapply funsig_main; eauto.
-Qed.
-*)
 Lemma match_final_states :
   forall st st' r,
     match_states st st' ->
